Work on egraph tooling

src/named/egraph/Proofs.v
@@ -70,6 +70,19 @@ Section __.
                  qt_unconstrained _ qt_tree
                  values_of_next_var choose_next_val relation db arg_map).
 
+    Notation add_and_check_ctx_cons :=
+      (add_and_check_ctx_cons eqn_set l qt_unconstrained trie_map qt_tree values_of_next_var choose_next_val relation db arg_map).
+
+    Notation Checker :=
+      (Checker eclass_map eqn_set).
+
+    Notation equality_saturation :=
+      (equality_saturation l qt_unconstrained trie_map qt_tree values_of_next_var choose_next_val relation db
+       arg_map).
+    
+    Notation resolve_checker' :=
+      (resolve_checker' l qt_unconstrained trie_map qt_tree values_of_next_var choose_next_val relation db arg_map).
+
     
     (*possibly poor naming*)
     Definition principal_sort c e : option sort :=
@@ -103,59 +116,183 @@ Section __.
         (*TODO: handle s_i up to uf_equiv? *)
         map.get g.(hashcons) (con_node n s_i) = Some i ->
         sort_in_egraph_at_index g i (scon n s).
+        
+    Definition is_ctx_of_egraph (g : egraph) (c : ctx) : Prop :=
+      Forall2 (fun '(x1,i) '(x2,t) => x1 = x2 /\ sort_in_egraph_at_index g i t)
+              g.(ectx) c.
 
-    Parameter is_ctx_of_egraph : egraph -> ctx -> Prop.
+    Section WithCtx.
+      Context (wfl : wf_lang l)
+              (c : ctx)
+              (wfc : wf_ctx l c).
 
-    Context (wfl : wf_lang l)
-            (c : ctx)
-            (wfc : wf_ctx l c).
+      Definition wf_egraph g (wf_ids : list idx) :=
+        all (fun x => In x wf_ids) (map snd g.(ectx))
+        /\ is_ctx_of_egraph g c
+        /\ (forall t1 t2 i,
+               sort_in_egraph_at_index g i t1 ->
+               sort_in_egraph_at_index g i t2 ->
+               In i wf_ids ->
+               eq_sort l c t1 t2)
+        /\ (forall e1 e2 t i,
+               term_in_egraph_at_index g i e1 ->
+               term_in_egraph_at_index g i e2 ->
+               In i wf_ids ->
+               (*TODO: does it matter whether the sort is in the egraph?*)
+               principal_sort c e1 = Some t ->
+               eq_term l c t e1 e2).
 
-    Definition wf_egraph g (wf_ids : list idx) :=
-      all (fun x => In x wf_ids) (map snd g.(ectx))
-      /\ is_ctx_of_egraph g c
-      /\ (forall t1 t2 i,
-             sort_in_egraph_at_index g i t1 ->
-             sort_in_egraph_at_index g i t2 ->
-             In i wf_ids ->
-             eq_sort l c t1 t2)
-      /\ (forall e1 e2 t i,
-             term_in_egraph_at_index g i e1 ->
-             term_in_egraph_at_index g i e2 ->
-             In i wf_ids ->
+      Lemma wf_egraph_sort_wf g wf_ids t i
+        : wf_egraph g wf_ids ->
+          sort_in_egraph_at_index g i t ->
+          In i wf_ids ->
+          wf_sort l c t.
+      Proof.
+        unfold wf_egraph.
+        basic_goal_prep.
+        eapply eq_sort_wf_l; eauto.
+      Qed.
+
+      
+      Lemma wf_egraph_term_wf g wf_ids e t i
+        : wf_egraph g wf_ids ->
+          term_in_egraph_at_index g i e ->
+          In i wf_ids ->
+          (*TODO: does it matter whether the sort is in the egraph?*)
+          principal_sort c e = Some t ->
+          wf_term l c e t.
+      Proof.
+        unfold wf_egraph.
+        basic_goal_prep.
+        eapply eq_term_wf_l; eauto.
+      Qed.
+
+      (*TODO: allow context extension?*)
+      Definition egraph_extends g1 g2 :=
+        (forall e i, term_in_egraph_at_index g1 i e ->
+                     term_in_egraph_at_index g2 i e)
+        /\ (forall t i, sort_in_egraph_at_index g1 i t ->
+                        sort_in_egraph_at_index g2 i t)
+        /\ (forall i j, union_find_equivalence g1.(id_equiv) i j ->
+                        union_find_equivalence g2.(id_equiv) i j).
+
+      Lemma egraph_extends_refl g : egraph_extends g g.
+      Proof.
+        unfold egraph_extends; intuition.
+      Qed.
+      
+    End WithCtx.
+
+    
+    Lemma empty_egraph_is_wf : wf_egraph [] empty_egraph [].
+    Proof.
+      unfold wf_egraph, is_ctx_of_egraph; basic_goal_prep; basic_utils_crush.
+    Qed.
+
+    
+    Definition indexed_terms_related c g i1 i2 :=
+      (forall t1 t2,
+          sort_in_egraph_at_index g i1 t1 ->
+          sort_in_egraph_at_index g i2 t2 ->
+          eq_sort l c t1 t2)
+      /\ (forall e1 e2 t,
+             term_in_egraph_at_index g i1 e1 ->
+             term_in_egraph_at_index g i2 e2 ->
              (*TODO: does it matter whether the sort is in the egraph?*)
              principal_sort c e1 = Some t ->
              eq_term l c t e1 e2).
-
-    Lemma wf_egraph_sort_wf g wf_ids t i
-      : wf_egraph g wf_ids ->
-        lookup_sort g t = Some i ->
-        In i wf_ids ->
-        wf_sort l c t.
-    Proof.
-      unfold wf_egraph.
-      basic_goal_prep.
-      eapply eq_sort_wf_l; eauto.
-    Qed.
+    
+    Definition up_to_checking {A} P (ch : Checker A) c
+      := forall g g' a eqns, ch g = (g', Some (a,eqns)) ->
+                            (forall i j, member eqns (i,j) = true ->
+                                         indexed_terms_related c g i j) ->
+                     P g' a.
 
     
-    Lemma wf_egraph_term_wf g wf_ids e t i i_t
-      : wf_egraph g wf_ids ->
-        lookup_term g e = Some (i,i_t) ->
-        In i wf_ids ->
-        lookup_sort g t = Some i_t ->
-        wf_term l c e t.
+    Lemma equality_saturation_sound {A} upd pred base fuel g g' (a:A) c good_ids
+      : (g', a) = equality_saturation upd pred base fuel g ->
+        wf_egraph c g good_ids ->
+        egraph_extends g g'
+        /\ wf_egraph c g' good_ids.
     Proof.
-      unfold wf_egraph.
-      basic_goal_prep.
-      eapply eq_term_wf_l; eauto.
+      revert g g' a base.
+      induction fuel; basic_goal_prep.
+      {
+        basic_utils_crush.
+        eapply egraph_extends_refl.
+      }
+      {
+        revert H1; case_match.
+        {
+          basic_utils_crush.
+          eapply egraph_extends_refl.
+        }
+        {
+          TODO: db reasoning
+        
+    Qed.
+      
+    
+    Lemma resolve_checker'_sound {A} g fuel ch g' (a : A) P c
+      : (g', Some a) = resolve_checker' ch fuel g ->
+        up_to_checking P ch c ->
+        P g' a.
+    Proof.
+      unfold resolve_checker'.
+      simpl.
+      case_match.
+      case_match; [| cbv; congruence].
+      destruct p.
+      case_match.
+      case_match; [| cbv; congruence].
+      intro H'; inversion H'; subst; clear H'.
+
+
+      
+      case_match.
+      
+    Qed.
+    
+    Lemma add_and_check_ctx_cons_sound i t c g g' good_ids
+      : (g',true) = add_and_check_ctx_cons i t g ->
+        wf_egraph c g good_ids ->
+        fresh i c ->
+        exists good_ids',
+          wf_egraph ((i,t)::c) g' (good_ids'++good_ids).
+    Proof.
+      unfold add_and_check_ctx_cons.
+      
+      case_match.
+      [| cbv; congruence].
+      case
     Qed.
 
+    Lemma check_ctx'_sound c g
+      : check_ctx' c = Some g -> exists good_ids, wf_egraph c g good_ids.
+      revert g.
+      induction c; basic_goal_prep; basic_utils_crush.
+      { eexists;now eapply empty_egraph_is_wf. }
+      {
+        revert H1.
+        case_match; [| cbv; congruence].
+        symmetry in HeqH1; apply use_compute_fresh in HeqH1.
+        case_match; [| cbv; congruence].
+        specialize (IHc e eq_refl); destruct IHc.
+        case_match.
+        destruct b; [| cbv; congruence].
+        basic_goal_prep; basic_utils_crush.
+        eapply add_and_check_ctx_cons_sound in HeqH2; eauto.
+        destruct HeqH2; eexists; eauto.
+      }
+    Qed.
+
+        
+        
+    Abort.
+    
     (*TODO: do I want a lookup_term function in defs?*)
     
     (*Properties I expect to hold:*)
-
-    Lemma empty_egraph_is_wf : wf_egraph empty_egraph.
-    Abort.
 
              
                       
