src/Utils/Gensym.v
@@ -1,0 +1,18 @@
+Set Implicit Arguments.
+Set Bullet Behavior "Strict Subproofs".
+
+Require List.
+From Utils Require Import Utils Natlike Monad.
+
+Section __.
+  Import StateMonad.
+
+  Context {S : Type}
+          `{Natlike S}.
+
+  Local Notation ST := (ST S).
+
+  Definition gensym : ST S :=
+    fun s => (succ s, s).
+
+End __.
